theories/lang/subst_map.v
@@ -1,0 +1,30 @@
+From stbor.lang Require Import expr_semantics.
+
+(** Substitution with a *map*, for the reflexivity proof. *)
+Fixpoint subst_map (xs : gmap string result) (e : expr) : expr :=
+  match e with
+  | Var y => if xs !! y is Some v then of_result v else Var y
+  | Val v => Val v
+  (* | Rec f xl e =>
+    Rec f xl $ if bool_decide (BNamed x ≠ f ∧ BNamed x ∉ xl) then subst_map xs e else e *)
+  | Call e el => Call (subst_map xs e) (map (subst_map xs) el)
+  | InitCall e => InitCall (subst_map xs e)
+  | EndCall e => EndCall (subst_map xs e)
+  | Place l tag T => Place l tag T
+  (* | App e1 el => App (subst_map xs e1) (map (subst_map xs) el) *)
+  | BinOp op e1 e2 => BinOp op (subst_map xs e1) (subst_map xs e2)
+  | Proj e1 e2 => Proj (subst_map xs e1) (subst_map xs e2)
+  | Conc e1 e2 => Conc (subst_map xs e1) (subst_map xs e2)
+  | Copy e => Copy (subst_map xs e)
+  | Write e1 e2 => Write (subst_map xs e1) (subst_map xs e2)
+  | Alloc T => Alloc T
+  | Free e => Free (subst_map xs e)
+  | Deref e T => Deref (subst_map xs e) T
+  | Ref e => Ref (subst_map xs e)
+  | Retag e kind => Retag (subst_map xs e) kind
+  | Let x1 e1 e2 =>
+      Let x1
+        (subst_map xs e1)
+        (subst_map (if x1 is BNamed s then delete s xs else xs) e2)
+  | Case e el => Case (subst_map xs e) (map (subst_map xs) el)
+  end.
